@prefix rdfs:   <http://www.w3.org/2000/01/rdf-schema#> .
@prefix rdf:    <http://www.w3.org/1999/02/22-rdf-syntax-ns#> .
@prefix owl:    <http://www.w3.org/2002/07/owl#> .
@prefix schema: <http://schema.org/> .
@prefix dct:    <http://purl.org/dc/terms/> .
@prefix voaf:   <http://purl.org/vocommons/voaf#> .
@prefix vann:   <http://purl.org/vocab/vann/> .
@prefix xsd:    <http://www.w3.org/2001/XMLSchema#> .
@prefix bow:    <https://betweenourworlds.org/ontology/> .
@prefix b:      <https://betweenourworlds.org/ontology> .

b: a owl:Ontology, voaf:Vocabulary, schema:Thing, schema:CreativeWork;
    rdfs:label                    "Between Our Worlds Ontology"@en;
    dct:title                     "Between Our Worlds Ontology"@en;
    rdfs:comment                  "The ontology focusses on the concepts of Anime."@en;
    dct:description               "The ontology focusses on the concepts of Anime."@en;
    rdfs:comment                  "De ontology focust op de concepten van Anime."@nl;
    dct:description               "De ontology focust op de concepten van Anime."@nl;
    schema:creator                <https://betweenourworlds.org/#bow>;
    dct:creator                   <https://betweenourworlds.org/#bow>;
    schema:dateCreated            "2017-07-14"^^schema:date;
    dct:issued                    "2017-07-14"^^xsd:date;
    schema:dateModified           "2018-09-27"^^schema:date;
    dct:modified                  "2018-09-27"^^xsd:date;
    owl:versionInfo               "1.2"^^xsd:decimal;
    vann:preferredNamespacePrefix "bow";
    vann:preferredNamespaceUri    "https://betweenourworlds.org/ontology/";
    schema:license                <http://creativecommons.org/publicdomain/zero/1.0> ;
    dct:license                   <http://creativecommons.org/publicdomain/zero/1.0> .

bow:Stream a rdfs:Class ;
    rdfs:label       "Stream" ;
    rdfs:comment     "The stream of an anime by a streaming service." ;
    rdfs:subClassOf  schema:Thing ;
    rdfs:isDefinedBy b: .

bow:Character a rdfs:Class ;
    rdfs:label       "Character";
    rdfs:comment     "A character that appears in an anime.";
    rdfs:subClassOf  schema:Thing;
    rdfs:isDefinedBy b: .

bow:object a owl:ObjectProperty ;
    rdfs:label       "object" ;
    rdfs:comment     "Similar to http://schema.org/object, but also for classes defined by this ontology." ;
    rdfs:domain      bow:Stream ;
    rdfs:isDefinedBy b: .

bow:providedBy a owl:ObjectProperty ;
    rdfs:label       "provided by" ;
    rdfs:comment     "Refers to the entity that provides the stream, i.e., the streaming service." ;
    rdfs:domain      bow:Stream ;
    rdfs:isDefinedBy b: .

bow:provides a owl:ObjectProperty ;
    rdfs:label       "provides" ;
    rdfs:comment     "Refers to the stream, i.e., the streaming of an anime provided by a streaming service." ;
    rdfs:range       bow:Stream ;
    owl:inverseOf    bow:providedBy ;
    rdfs:isDefinedBy b: .

bow:character a owl:ObjectProperty ;
    rdfs:label       "has character" ;
    rdfs:comment     "Links an entity, e.g., anime, to a character that appears in it." ;
    rdfs:range       bow:Character ;
    rdfs:isDefinedBy b: .